theories/FOL/Reductions/PCPb_to_binZF.v
@@ -8,6 +8,7 @@ Local Set Implicit Arguments.
 Local Unset Strict Implicit.
 
 Require Import Equations.Equations.
+Require Import Morphisms.
 
 Local Notation vec := Vector.t.
 
@@ -223,8 +224,38 @@ Section Model.
     - intros d Hd. exists (σ d). split; try now apply M_om1. intros d'. now apply sigma_el.
   Qed.
 
+  Instance set_equiv_equiv' :
+    Equivalence set_equiv.
+  Proof.
+    now apply set_equiv_equiv.
+  Qed.
+
+  Instance set_equiv_elem' :
+    Proper (set_equiv ==> set_equiv ==> iff) set_elem.
+  Proof.
+    now apply set_equiv_elem.
+  Qed.
+
+  Instance set_equiv_sub' :
+    Proper (set_equiv ==> set_equiv ==> iff) set_sub.
+  Proof.
+    now apply set_equiv_sub.
+  Qed.
+
+  Instance equiv_union' :
+    Proper (set_equiv ==> set_equiv) union.
+  Proof.
+    now apply equiv_union.
+  Qed.
+
+  Instance equiv_power' :
+    Proper (set_equiv ==> set_equiv) power.
+  Proof.
+    now apply equiv_power.
+  Qed.
+
   Lemma rm_const_tm_sat (rho : nat -> V) (t : term) x :
-    (x .: rho) ⊨ embed (rm_const_tm t) <-> x ≡ eval rho t.
+    (x .: rho) ⊨ embed (rm_const_tm t) <-> set_equiv x (eval rho t).
   Proof.
     induction t in x |- *; try destruct F; cbn; split;
     try rewrite (vec_inv1 v); try rewrite (vec_inv2 v); cbn.
@@ -234,42 +265,49 @@ Section Model.
       intros H. apply M_ext; trivial; intros y Hy; exfalso; intuition.
       now apply M_eset in Hy. 
     - rewrite (vec_nil_eq (Vector.map (eval rho) v)).
-      intros d. (*now apply M_eset.
+      change (set_equiv x ∅ -> forall d : V, set_elem d x -> False).
+      intros H d. rewrite H. now apply M_eset.
     - intros (y & Hy & z & Hz & H).
-      rewrite embed_sshift, sat_sshift1, IH in Hy; try apply in_hd. subst.
-      rewrite embed_sshift, sat_sshift2, IH in Hz; try apply in_hd_tl. subst.
+      rewrite embed_sshift, sat_sshift1, IH in Hy; try apply in_hd.
+      rewrite embed_sshift, sat_sshift2, IH in Hz; try apply in_hd_tl.
       apply M_ext; trivial.
-      + intros a Ha % H. rewrite !eq_equiv in Ha. now apply M_pair.
-      + intros a Ha % M_pair; trivial. apply H. now rewrite !eq_equiv.
+      + intros a Ha % H. rewrite !eq_equiv in Ha. apply M_pair; trivial.
+        rewrite <- Hy, <- Hz. tauto.
+      + intros a Ha % M_pair; trivial. apply H. rewrite !eq_equiv.
+        rewrite <- Hy, <- Hz in Ha. tauto.
     - exists (eval rho (Vector.hd v)).
-      rewrite embed_sshift, sat_sshift1, IH; try apply in_hd. split; trivial.
+      rewrite embed_sshift, sat_sshift1, IH; try apply in_hd. split; try reflexivity.
       exists (eval rho (Vector.hd (Vector.tl v))).
-      rewrite embed_sshift, sat_sshift2, IH; try apply in_hd_tl. split; trivial.
-      intros d. rewrite !eq_equiv. now apply M_pair.
-    - intros (y & Hy & H).
-      rewrite embed_sshift, sat_sshift1, IH in Hy; try apply in_hd. subst.
-      apply M_ext; trivial.
-      + intros y Hy % H. now apply M_union.
-      + intros y Hy % M_union; trivial. now apply H.
+      rewrite embed_sshift, sat_sshift2, IH; try apply in_hd_tl. split; try reflexivity.
+      change (forall d, (set_elem d x -> d ≈ eval rho (Vector.hd v) \/ d ≈ eval rho (Vector.hd (Vector.tl v))) /\ 
+              (d ≈ eval rho (Vector.hd v) \/ d ≈ eval rho (Vector.hd (Vector.tl v)) -> set_elem d x)).
+      intros d. rewrite !eq_equiv, H. now apply M_pair.
+    - intros (y & Hy & H). rewrite embed_sshift, sat_sshift1, IH in Hy; try apply in_hd.
+      change (set_equiv x (union (eval rho (Vector.hd v)))). rewrite <- Hy. apply M_ext; trivial.
+      + intros z Hz % H. now apply M_union.
+      + intros z Hz % M_union; trivial. now apply H.
+    - exists (eval rho (Vector.hd v)). rewrite embed_sshift, sat_sshift1, IH; try apply in_hd. split; try reflexivity.
+      change (forall d, (set_elem d x -> exists d0 : V, d0 ∈ eval rho (Vector.hd v) /\ d ∈ d0) /\
+              ((exists d0 : V, d0 ∈ eval rho (Vector.hd v) /\ d ∈ d0) -> set_elem d x)).
+      intros d. rewrite H. now apply M_union.
+    - intros (y & Hy & H). rewrite embed_sshift, sat_sshift1, IH in Hy; try apply in_hd.
+      change (set_equiv x (power (eval rho (Vector.hd v)))). rewrite <- Hy. apply M_ext; trivial.
+      + intros z Hz. now apply M_power, H.
+      + intros z Hz. now apply H, M_power.
     - exists (eval rho (Vector.hd v)).
-      rewrite embed_sshift, sat_sshift1, IH; try apply in_hd. split; trivial.
-      intros d. now apply M_union.
-    - intros (y & Hy & H).
-      rewrite embed_sshift, sat_sshift1, IH in Hy; try apply in_hd. subst.
-      apply M_ext; trivial.
-      + intros y Hy. now apply M_power, H.
-      + intros y Hy. now apply H, M_power.
-    - exists (eval rho (Vector.hd v)).
-      rewrite embed_sshift, sat_sshift1, IH; try apply in_hd. split; trivial.
-      intros d. now apply M_power.
+      rewrite embed_sshift, sat_sshift1, IH; try apply in_hd. split; try reflexivity.
+      change (forall d, (set_elem d x -> d ⊆ eval rho (Vector.hd v)) /\ (d ⊆ eval rho (Vector.hd v) -> set_elem d x)).
+      intros d. rewrite H. now apply M_power.
     - rewrite (vec_nil_eq (Vector.map (eval rho) v)). intros [H1 H2]. apply M_ext; trivial.
-      + apply H2. apply (inductive_sat_om rho).
-      + apply M_om2; trivial. apply inductive_sat with rho. apply H1.
+      + unfold set_sub. apply H2. apply (inductive_sat_om rho).
+      + unfold set_sub. apply M_om2; trivial. apply inductive_sat with rho. apply H1.
     - rewrite (vec_nil_eq (Vector.map (eval rho) v)). split.
-      + apply (inductive_sat_om rho).
-      + intros d Hd. apply M_om2; trivial. apply inductive_sat with rho. apply Hd.
-  Qed.*)
-  Admitted.
+      + change ((exists d : V, (forall d0 : V, d0 ∈ d -> False) /\ set_elem d x) /\ (forall d : V, set_elem d x
+            -> exists d0 : V, (forall d1 : V, (d1 ∈ d0 -> d1 ∈ d \/ d1 ≈ d) /\ (d1 ∈ d \/ d1 ≈ d -> d1 ∈ d0)) /\ set_elem d0 x)).
+        setoid_rewrite H. apply (inductive_sat_om rho).
+      + intros d Hd. change (set_sub x d). rewrite H. unfold set_sub.
+        apply M_om2; trivial. apply inductive_sat with rho. apply Hd.
+  Qed.
 
   Lemma rm_const_sat (rho : nat -> V) (phi : form) :
     rho ⊨ phi <-> rho ⊨ embed (rm_const_fm phi).
